pcuic/theories/PCUICInst.v
@@ -89,27 +89,6 @@ Proof.
 Qed.
 Hint Rewrite rename_context_inst_context : sigma.
 
-Lemma subst1_inst :
-forall t n u,
-  t{ n := u } = t.[⇑^n (u ⋅ ids)].
-Proof.
-intros t n u.
-unfold subst1. rewrite subst_inst.
-eapply inst_ext. intro i.
-unfold Upn, subst_compose, subst_consn.
-destruct (Nat.ltb_spec0 i n).
-- rewrite -> nth_error_idsn_Some by assumption. reflexivity.
-- rewrite -> nth_error_idsn_None by lia.
-  rewrite idsn_length.
-  destruct (Nat.eqb_spec (i - n) 0).
-  + rewrite e. simpl. reflexivity.
-  + replace (i - n) with (S (i - n - 1)) by lia. simpl.
-    destruct (i - n - 1) eqn: e.
-    * simpl. reflexivity.
-    * simpl. reflexivity.
-Qed.
-(* Hint Rewrite @subst1_inst : sigma. *)
-
 Lemma subst10_inst a b τ : b {0 := a}.[τ] = (b.[⇑ τ] {0 := a.[τ]}).
 Proof.
   unfold subst10. simpl. rewrite !subst_inst.
@@ -202,34 +181,6 @@ Proof.
         rewrite Nat.sub_diag in hnth. simpl in hnth. congruence.
 Qed.
 
-Lemma inst_closed σ k t : closedn k t -> t.[⇑^k σ] = t.
-Proof.
-  intros Hs.
-  induction t in σ, k, Hs |- * using term_forall_list_ind; intros; sigma;
-    simpl in *;
-    rewrite -> ?map_map_compose, ?compose_on_snd, ?compose_map_def, ?map_branch_map_branch,
-      ?map_length, ?Nat.add_assoc in *;
-      unfold test_def, map_branch, test_branch, test_predicate in *; simpl in *; eauto with all;
-    simpl closed in *; repeat (rtoProp; f_equal; solve_all); try change_Sk.
-    
-  - revert Hs.
-    unfold Upn.
-    elim (Nat.ltb_spec n k); intros. simpl in *.
-    destruct (subst_consn_lt (l := idsn k) (i := n)) as [t [Heq Heq']].
-    + now rewrite idsn_length //.
-    + now rewrite idsn_lt in Heq.
-    + discriminate.
-  - specialize (IHt2 σ (S k) H0). rewrite -{2}IHt2. now sigma.
-  - specialize (IHt2 σ (S k) H0). rewrite -{2}IHt2. now sigma.
-  - specialize (IHt3 σ (S k) H0). rewrite -{2}IHt3. now sigma.
-  - specialize (e σ (#|pcontext p| + k)). rewrite -{2}e; now sigma.
-  - specialize (a σ (#|bcontext x| + k)). destruct x; simpl in *. f_equal.
-    now rewrite -{2}a; sigma.
-  - rtoProp. specialize (b0 σ (#|m| + k) H0). eapply map_def_id_spec; auto.
-    revert b0. now sigma.
-  - rtoProp. specialize (b0 σ (#|m| + k) H0). eapply map_def_id_spec; auto.
-    revert b0. now sigma.
-Qed.
 
 Lemma inst_decl_closed :
   forall σ k d,
